books/kestrel/axe/risc-v/registers.lisp
@@ -1,0 +1,102 @@
+; Normal forms for register operations
+;
+; Copyright (C) 2025 Kestrel Institute
+;
+; License: A 3-clause BSD license. See the file books/3BSD-mod.txt.
+;
+; Author: Eric Smith (eric.smith@kestrel.edu)
+
+;;;;;;;;;;;;;;;;;;;;;;;;;;;;;;;;;;;;;;;;;;;;;;;;;;;;;;;;;;;;;;;;;;;;;;;;;;;;;;;;
+
+(in-package "R")
+
+;; TODO: Consider adding 32 to the names of the functions in this file (or
+;; making separate packages for 32-bit and 64-bit RISC-V proofs).  Note that
+;; the functions defined in this file are analogous to the functions used by
+;; Axe for x86 reasoning (except for the memory size).
+
+(include-book "portcullis")
+(include-book "risc-v-rules")
+(include-book "kestrel/risc-v/specialized/states32" :dir :system)
+(include-book "kestrel/bv/bvchop-def" :dir :system)
+(local (include-book "kestrel/bv/bvchop" :dir :system))
+
+(local
+  (defthm unsigned-byte-p-when-ubyte32p
+    (implies (ubyte32p x)
+             (unsigned-byte-p 32 x))
+    :hints (("Goal" :in-theory (enable ubyte32p)))))
+
+;; Gets the value of register N.
+(defund reg (n stat)
+  (declare (xargs :guard (and (posp n)
+                              (< n 31)
+                              (stat32ip stat))
+                  :guard-hints (("Goal" :in-theory (enable ubyte5p)))))
+  (read32-xreg-unsigned n stat))
+
+(defthm unsigned-byte-p-of-reg (unsigned-byte-p 32 (reg n stat)) :hints (("Goal" :in-theory (enable reg))))
+
+;; Introduces REG.
+(defthmd read32-xreg-unsigned-becomes-reg
+  (equal (read32-xreg-unsigned n stat)
+         (reg n stat))
+  :hints (("Goal" :in-theory (enable reg))))
+
+;; todo: reg-of-0
+
+;;;;;;;;;;;;;;;;;;;;;;;;;;;;;;;;;;;;;;;;;;;;;;;;;;;;;;;;;;;;;;;;;;;;;;;;;;;;;;;;
+
+;; Sets the value of register N.
+(defund set-reg (n val stat)
+  (declare (xargs :guard (and (posp n)
+                              (< n 31)
+                              (unsigned-byte-p 32 val)
+                              (stat32ip stat))
+                  :guard-hints (("Goal" :in-theory (enable ubyte5p)))))
+  (write32-xreg n val stat))
+
+;; writing to "register 0" has no effect
+(defthm set-reg-of-0
+  (implies (stat32ip stat) ; too bad
+           (equal (set-reg 0 val stat)
+                  stat))
+  :hints (("Goal" :in-theory (enable set-reg))))
+
+;; Introduces set-reg.
+(defthmd write32-xreg-becomes-set-reg
+  (equal (write32-xreg n val stat)
+         (set-reg n val stat))
+  :hints (("Goal" :in-theory (enable set-reg))))
+
+(defthm error32p-of-set-reg (equal (error32p (set-reg n val stat)) (error32p stat)) :hints (("Goal" :in-theory (enable set-reg))))
+(defthm read32-pc-of-set-reg (equal (read32-pc (set-reg n val stat)) (read32-pc stat)) :hints (("Goal" :in-theory (enable set-reg))))
+
+;; both cases (the register numbers should usually be constants)
+(defthm reg-of-set-reg
+  (implies (and (posp n1)
+                (posp n2)
+                (< n1 32)
+                (< n2 32))
+           (equal (reg n1 (set-reg n2 val stat))
+                  (if (equal n1 n2)
+                      (bvchop 32 val)
+                    (reg n1 stat))))
+  :hints (("Goal" :in-theory (enable reg set-reg ubyte5-fix ubyte5p bvchop))))
+
+(defthm reg-of-write32-pc (equal (reg n (write32-pc pc stat)) (reg n stat)) :hints (("Goal" :in-theory (enable reg))))
+
+;;;;;;;;;;;;;;;;;;;;;;;;;;;;;;;;;;;;;;;;;;;;;;;;;;;;;;;;;;;;;;;;;;;;;;;;;;;;;;;;
+
+;; register aliases (we plan to keep these enabled):
+(defund x1 (stat) (declare (xargs :guard (stat32ip stat))) (reg 1 stat))
+(defund x2 (stat) (declare (xargs :guard (stat32ip stat))) (reg 2 stat))
+(defund x8 (stat) (declare (xargs :guard (stat32ip stat))) (reg 8 stat))
+(defund x10 (stat) (declare (xargs :guard (stat32ip stat))) (reg 10 stat))
+(defund x11 (stat) (declare (xargs :guard (stat32ip stat))) (reg 11 stat))
+
+;; register aliases (we plan to keep these enabled):
+(defun ra (stat) (declare (xargs :guard (stat32ip stat))) (x1 stat))
+(defun sp (stat) (declare (xargs :guard (stat32ip stat))) (x2 stat))
+(defun a0 (stat) (declare (xargs :guard (stat32ip stat))) (x10 stat))
+(defun a1 (stat) (declare (xargs :guard (stat32ip stat))) (x11 stat))
