books/kestrel/axe/risc-v/acl2-customization.lsp
@@ -1,0 +1,19 @@
+; ACL2 customization file for this dir
+;
+; Copyright (C) 2025 Kestrel Institute
+;
+; License: A 3-clause BSD license. See the file books/3BSD-mod.txt.
+;
+; Author: Eric Smith (eric.smith@kestrel.edu)
+
+;;;;;;;;;;;;;;;;;;;;;;;;;;;;;;;;;;;;;;;;;;;;;;;;;;;;;;;;;;;;;;;;;;;;;;;;;;;;;;;;
+
+;; load the user's acl2-customization.lsp, if any:
+(ld "~/acl2-customization.lsp" :ld-missing-input-ok t)
+
+(include-book "kestrel/risc-v/portcullis" :dir :system)
+
+(ld "package.lsp")
+(in-package "R")
+
+(reset-prehistory)
